session1/training1.dfy
@@ -121,7 +121,7 @@ ensures true
  *  Check whether a sequence of letters is a palindrom.
  *
  *  Try to:
- *  1. write the algorithm to determine whether a string is a palindrom
+ *  1. write the algorithm to determine whether a string is a palindrome
  *  2. write the ensures clauses that specify the palidrom properties
  *  3. verify algorithm. 
  *
@@ -129,7 +129,7 @@ ensures true
  *  a[i..j] is (a seq) with the first j elements minus the first i
  *  a[0.. |a| - 1] is same as a.  
  */
-method isPalindrom(a: seq<char>) returns (b: bool) 
+method isPalindrome(a: seq<char>) returns (b: bool) 
 {
     return true;
 }
@@ -181,20 +181,20 @@ method Main() {
    
     //  run palindrom
     var s1 := ['a'];
-    var r1 := isPalindrom(s1);
-    print "[", s1, "]", " is a palindrom? ", r1, " \n";
+    var r1 := isPalindrome(s1);
+    print "is [", s1, "]", " a isPalindrome? ", r1, " \n";
 
     s1 := [];
-    r1 := isPalindrom(s1);
-    print "[", s1, "]", " is a palindrom? ", r1, " \n";
+    r1 := isPalindrome(s1);
+    print "is [", s1, "]", " a isPalindrome? ", r1, " \n";
 
     s1 := ['a', 'b'];
-    r1 := isPalindrom(s1);
-    print "[", s1, "]", " is a palindrom? ", r1, " \n";
+    r1 := isPalindrome(s1);
+    print "is [", s1, "]", " a isPalindrome? ", r1, " \n";
 
     s1 := ['a', 'b', 'a'];
-    r1 := isPalindrom(s1);
-    print "[", s1, "]", " is a palindrom? ", r1, " \n";
+    r1 := isPalindrome(s1);
+    print "is [", s1, "]", " a isPalindrome? ", r1, " \n";
 
     // run unique
     var i := [0,1,3,3,5,5,7];
